ulib/LowStar.RST.Array.fst
@@ -15,6 +15,8 @@
 *)
 module LowStar.RST.Array
 
+friend LowStar.Array
+
 let index (#a:Type) (b:A.array a) (i:UInt32.t) = reveal_array(); A.index b i
 
 let upd (#a:Type) (b:A.array a) (i:UInt32.t) (v:a) =
@@ -119,3 +121,165 @@ let glue #a b b1 b2 =
   (**) A.loc_union_is_split_into b b1 b2
 
 #pop-options
+
+
+
+abstract
+let full_array_view (#a:Type) (b:A.array a) : view (varray a) =
+  reveal_view ();
+  let fp = Ghost.hide (A.loc_freed_mreference b.A.content) in
+  let inv h =
+    A.live h b /\ constant_perm_seq h b
+  in
+  let sel (h: HS.mem) : GTot (varray a) = { s = A.as_seq h b; p = A.get_perm h b 0 } in
+  {
+    fp = fp;
+    inv = inv;
+    sel = sel
+  }
+
+
+let full_array_resource (#a:Type) (b:A.array a) =
+  as_resource (full_array_view b)
+
+let promote (#a:Type) (b:A.array a) : RST unit
+  (full_array_resource b)
+  (fun _ -> array_resource b)
+  (fun _ -> True)
+  (fun _ _ _ -> True)
+  = 
+  let h0 = HST.get() in
+  reveal_array();
+  reveal_rst_inv();
+  reveal_modifies();
+  // assume     (forall frame .
+  //     A.loc_disjoint frame (A.loc_array b) /\
+  //     A.loc_includes (A.loc_not_unused_in h0) frame
+  //     ==>
+  //     A.loc_disjoint frame (A.loc_freed_mreference b.A.content) /\
+  //     A.loc_includes (A.loc_not_unused_in h0) frame);
+
+//  assume (modifies (array_resource b) (full_array_resource b) h0 h0);
+  ()
+
+let test (#a:Type) (b:A.array a) (v:a): RST unit
+  (full_array_resource b)
+  (fun _ -> full_array_resource b)
+  (fun h0 -> P.allows_write (sel (full_array_view b) h0).p)
+  (fun _ _ _ -> True)
+  =
+  reveal_array();
+  reveal_rst_inv();
+  reveal_modifies();
+  upd b 0ul v;
+  ()
+
+assume
+val arr_free (#a: Type) (b: A.array a) : HST.ST unit
+  (requires (fun h0 -> A.writeable h0 b /\ A.live  h0 b /\ A.freeable b))
+  (ensures (fun h0 _ h1 ->
+    Map.domain (HS.get_hmap h1) `Set.equal` Map.domain (HS.get_hmap h0) /\
+    (HS.get_tip h1) == (HS.get_tip h0) /\
+    A.modifies (A.loc_freed_mreference b.A.content) h0 h1 /\
+    HS.live_region h1 (A.frameOf b)
+  ))
+
+let full_free (#a:Type) (b:A.array a)
+  : RST unit (full_array_resource b)
+             (fun _ -> empty_resource)
+             (fun h0 -> A.freeable b /\ P.allows_write (sel (array_view b) h0).p)
+             (fun _ _ _ -> True)
+  =  (**) reveal_array();
+  (**) reveal_empty_resource();
+  (**) reveal_rst_inv();
+  (**) reveal_modifies();
+  arr_free b
+
+val arr_alloc (#a:Type0) (init:a) (len:UInt32.t)
+  : ST (A.array a)
+       (requires fun _ -> UInt32.v len > 0)
+       (ensures fun h0 b h1 ->
+         A.modifies A.loc_none h0 h1 /\
+         A.fresh_loc (A.loc_freed_mreference b.A.content) h0 h1 /\
+         A.writeable h1 b /\
+         A.freeable b /\
+         A.as_seq h1 b == Seq.create (UInt32.v len) init)
+
+let arr_alloc #a init len =
+  let perm_map_pid = Ghost.hide (
+    let (vp, pid) = LowStar.Permissions.new_value_perms init true in
+    ((vp <: LowStar.Permissions.perms_rec a), Ghost.hide pid)
+  ) in
+  let v = (init, Ghost.hide (fst (Ghost.reveal perm_map_pid))) in
+  let s = Seq.create (UInt32.v len) v in
+  (**) let h0 = HST.get() in
+  let content = HST.ralloc_mm HS.root s in
+  (**) let h1 = HST.get() in
+  (**) MG.modifies_ralloc_post #A.ucell #A.cls HS.root s h0 content h1;
+  let b = A.Array len content 0ul len (snd (Ghost.reveal perm_map_pid)) in
+  (**) assert (Seq.equal (A.as_seq h1 b) (Seq.create (UInt32.v len) init));
+  b
+
+let full_alloc (#a:Type) (init:a) (len:UInt32.t)
+  : RST (A.array a)
+        (empty_resource)
+        (fun b -> full_array_resource b)
+        (fun _ -> UInt32.v len > 0)
+        (fun _ b h1 ->
+        A.freeable b /\
+        (sel (array_view b) h1).s == Seq.create (UInt32.v len) init /\
+        (sel (array_view b) h1).p = FStar.Real.one
+        )
+  =   (**) reveal_array();
+  (**) reveal_rst_inv();
+  (**) reveal_modifies();
+  let b = arr_alloc init len in
+  // (**) let h1 = HST.get () in
+  // (**) assert(forall (i:nat{i < A.vlength #a b}). A.get_perm #a h1 b i = FStar.Real.one); // Find out how to trigger that
+  // (**) A.loc_includes_adresses_loc_array #a b true;
+  b
+
+let frame_full_pre (#a:Type) (b:A.array a) (res:resource) (pre:r_pre (array_resource b <*> res)) 
+  (h:imem (inv (full_array_resource b <*> res)))
+  = 
+  reveal_array();
+  reveal_star();
+  pre h /\
+  sel (array_view b) h == sel (full_array_view b) h
+
+let frame_full_post(#t:Type)
+                   (#a:Type) 
+                   (b:A.array a)
+                   (res0:resource) 
+                   (res1:t -> resource)
+                   (pre:r_pre (array_resource b <*> res0)) 
+                   (post:r_post (array_resource b <*> res0) t (fun x -> array_resource b <*> res1 x))
+                   (h0:imem (inv (full_array_resource b <*> res0)))
+                   (x:t)
+                   (h1:imem (inv (full_array_resource b <*> res1 x)))
+    = reveal_array();
+      reveal_star();
+      post h0 x h1 /\
+      sel (array_view b) h1 == sel (full_array_view b) h1
+
+let frame_full_array (#t:Type) (#a:Type) (b:A.array a)
+    (res0:resource)
+    (res1:t -> resource)
+    (#pre:r_pre (array_resource b <*> res0))
+    (#post:r_post (array_resource b <*> res0) t (fun x -> array_resource b <*> res1 x))
+    ($f:unit -> RST t (array_resource b <*> res0) (fun x -> array_resource b <*> res1 x) pre post) 
+    : RST t
+      (full_array_resource b <*> res0)
+      (fun x -> full_array_resource b <*> res1 x)
+      (frame_full_pre b res0 pre)
+      (frame_full_post b res0 res1 pre post)
+   = reveal_modifies();
+     reveal_rst_inv();
+     reveal_array();
+     reveal_star();
+     let h0 = HST.get() in
+     let x = f() in
+     let h1 = HST.get() in
+     A.loc_includes_disjoint_elim (as_loc (fp (res1 x))) (A.loc_array b) (A.loc_union (as_loc (fp res0)) (A.loc_unused_in h0));
+     A.unused_in_not_unused_in_disjoint_2 (A.loc_unused_in h0) (A.loc_not_unused_in h0) (A.loc_unused_in h0) (A.loc_not_unused_in h0) h0;
+     x
